theories/int_or_ptr/vst/verif/vsu.v
@@ -1,0 +1,20 @@
+From VST Require Import floyd.proofauto.
+From VST Require Import floyd.VSU.
+
+From appliedfm Require Import int_or_ptr.vst.clightgen.int_or_ptr.
+From appliedfm Require Import int_or_ptr.vst.spec.spec.
+From appliedfm Require Import int_or_ptr.vst.verif.verif.
+
+#[local] Existing Instance NullExtension.Espec.
+
+Lemma VSU: VSU [] VSUspec.imports ltac:(QPprog prog) VSUspec.exports emp.
+Proof.
+mkVSU prog VSUspec.all.
+- solve_SF_internal body_int_or_ptr__sizeof.
+- solve_SF_internal body_int_or_ptr__alignof.
+- solve_SF_internal body_int_or_ptr__is_int.
+- solve_SF_internal body_int_or_ptr__to_int.
+- solve_SF_internal body_int_or_ptr__to_ptr.
+- solve_SF_internal body_int_or_ptr__of_int.
+- solve_SF_internal body_int_or_ptr__of_ptr.
+Qed.
